proofmode/invariants.v
@@ -9,23 +9,23 @@ Implicit Types N : namespace.
 Implicit Types P Q R : iProp Λ Σ.
 
 Lemma tac_inv_fsa {A} (fsa : FSA Λ Σ A) fsaV Δ Δ' E N i P Q Φ :
-  FSASplit Q E fsa fsaV Φ →
+  IsFSA Q E fsa fsaV Φ →
   fsaV → nclose N ⊆ E → (of_envs Δ ⊢ inv N P) →
   envs_app false (Esnoc Enil i (▷ P)) Δ = Some Δ' →
   (Δ' ⊢ fsa (E ∖ nclose N) (λ a, ▷ P ★ Φ a)) → Δ ⊢ Q.
 Proof.
-  intros ????? HΔ'. rewrite -(fsa_split Q) -(inv_fsa fsa _ _ P) //.
+  intros ????? HΔ'. rewrite (is_fsa Q) -(inv_fsa fsa _ _ P) //.
   rewrite // -always_and_sep_l. apply and_intro; first done.
   rewrite envs_app_sound //; simpl. by rewrite right_id HΔ'.
 Qed.
 
 Lemma tac_inv_fsa_timeless {A} (fsa : FSA Λ Σ A) fsaV Δ Δ' E N i P Q Φ :
-  FSASplit Q E fsa fsaV Φ →
+  IsFSA Q E fsa fsaV Φ →
   fsaV → nclose N ⊆ E → (of_envs Δ ⊢ inv N P) → TimelessP P →
   envs_app false (Esnoc Enil i P) Δ = Some Δ' →
   (Δ' ⊢ fsa (E ∖ nclose N) (λ a, P ★ Φ a)) → Δ ⊢ Q.
 Proof.
-  intros ?????? HΔ'. rewrite -(fsa_split Q) -(inv_fsa fsa _ _ P) //.
+  intros ?????? HΔ'. rewrite (is_fsa Q) -(inv_fsa fsa _ _ P) //.
   rewrite // -always_and_sep_l. apply and_intro, wand_intro_l; first done.
   trans (|={E ∖ N}=> P ★ Δ)%I; first by rewrite pvs_timeless pvs_frame_r.
   apply (fsa_strip_pvs _).
@@ -36,7 +36,7 @@ End invariants.
 
 Tactic Notation "iInvCore" constr(N) "as" constr(H) :=
   eapply tac_inv_fsa with _ _ _ _ N H _ _;
-    [let P := match goal with |- FSASplit ?P _ _ _ _ => P end in
+    [let P := match goal with |- IsFSA ?P _ _ _ _ => P end in
      apply _ || fail "iInv: cannot viewshift in goal" P
     |try fast_done (* atomic *)
     |done || eauto with ndisj (* [eauto with ndisj] is slow *)
@@ -62,7 +62,7 @@ Tactic Notation "iInv" constr(N) "as" "{" simple_intropattern(x1)
 
 Tactic Notation "iInvCore>" constr(N) "as" constr(H) :=
   eapply tac_inv_fsa_timeless with _ _ _ _ N H _ _;
-    [let P := match goal with |- FSASplit ?P _ _ _ _ => P end in
+    [let P := match goal with |- IsFSA ?P _ _ _ _ => P end in
      apply _ || fail "iInv: cannot viewshift in goal" P
     |try fast_done (* atomic *)
     |done || eauto with ndisj (* [eauto with ndisj] is slow *)
